Thesis/Definitions/NaturalSemantics.lean
@@ -20,33 +20,33 @@ inductive big_step : Stmt → State → State → Prop where
       big_step Stmt.skip s s
 
   -- [compₙₛ] rule (given ⟨S₁, s⟩ → s' and ⟨S₂, s'⟩ → s'' we produce ⟨S, s⟩ → s'')
-  | seq {S₁ S₂ s s' s''} :
-      big_step S₁ s  s'  →
-      big_step S₂ s' s'' →
+  | seq {S₁ S₂ s s' s''}
+    (h_left  : big_step S₁ s  s')
+    (h_right : big_step S₂ s' s'') :
       big_step (Stmt.sequence S₁ S₂) s s''
 
   -- [ifᵗᵗₙₛ] rule (given ⟨S₁, s⟩ → s' and 𝓑⟦b⟧ s = true we produce ⟨S, s⟩ → s')
   | if_true {b S₁ S₂ s s'} :
-      𝓑⟦b⟧ s = true →
-      big_step S₁ s s' →
+    (h_cond : 𝓑⟦b⟧ s = true) →
+    (h_then : big_step S₁ s s') →
       big_step (Stmt.cond b S₁ S₂) s s'
 
   -- [ifᶠᶠₙₛ] rule (given ⟨S₂, s⟩ → s' and 𝓑⟦b⟧ s = false we produce ⟨S, s⟩ → s')
-  | if_false {b S₁ S₂ s s'} :
-      𝓑⟦b⟧ s = false →
-      big_step S₂ s s' →
+  | if_false {b S₁ S₂ s s'}
+    (h_cond : 𝓑⟦b⟧ s = false)
+    (h_else : big_step S₂ s s') :
       big_step (Stmt.cond b S₁ S₂) s s'
 
   -- [whileᵗᵗₙₛ] rule (given ⟨S', s⟩ → s', ⟨while b do S', s'⟩ → s'' and 𝓑⟦b⟧ s = true we produce ⟨S, s⟩ → s'')
-  | while_true {b S s s' s''} :
-      𝓑⟦b⟧ s = true →
-      big_step S s s' →
-      big_step (Stmt.loop b S) s' s'' →
+  | while_true {b S s s' s''}
+    (h_cond : 𝓑⟦b⟧ s = true)
+    (h_step : big_step S s s')
+    (h_rest : big_step (Stmt.loop b S) s' s'') :
       big_step (Stmt.loop b S) s s''
 
   -- [whileᶠᶠₙₛ] rule (given 𝓑⟦b⟧ s = false we produce ⟨S, s⟩ → s)
-  | while_false {b S' s} :
-      𝓑⟦b⟧ s = false →
+  | while_false {b S' s}
+    (h_cond : 𝓑⟦b⟧ s = false) :
       big_step (Stmt.loop b S') s s
 
 -- Define the standard Nielson & Nielson notation
